**Expression Syntax: `$…$, $$…$$`**

`$A^T_S = B$` --> $A^T_S = B$  
`$$A^T_S = B$$` --> $$A^T_S = B$$  

`$\sqrt{ab}$` --> $\sqrt{ab}$  
`$$\sqrt{ab}$$` --> $$\sqrt{ab}$$

_Pipe Table_

|   Expression    |   Rendering   |
| :-------------: | :-----------: |
|  `$A^T_S = B$`  |  $A^T_S = B$  |
| `$$A^T_S = B$$` | $$A^T_S = B$$ |
|  `$\sqrt{ab}$`  |  $\sqrt{ab}$  |
| `$$\sqrt{ab}$$` | $$\sqrt{ab}$$ |

_html `<table>`_

<table style="width:100%; font-family: monospace;">
<tr>
  <th>Expression</th>
  <th>Rendering</th>
</tr>
<tr>
  <td>`$A^T_S = B$`</td>
  <td>$A^T_S = B$</td>
</tr>
<tr>
  <td>`$$A^T_S = B$$`</td>
  <td>$$A^T_S = B$$</td>
</tr>
</table>

_`<div>`_

<div>$A^T_S = B$</div>    
<div>$$A^T_S = B$$</div>  

----------

**Expression Syntax: `\\(…\\), \\[…\\]`**  


`\\(A^T_S = B\\)` --> \\(A^T_S = B\\)  
`\\[A^T_S = B\\]` --> \\[A^T_S = B\\]  

`\\(\sqrt{ab}\\)` --> \\(\sqrt{ab}\\)  
`\\[\sqrt{ab}\\]` --> \\[\sqrt{ab}\\]  

_Pipe Table_

|     Expression      |     Rendering     |
| :-----------------: | :---------------: |
| `\\( A^T_S = B \\)` | \\( A^T_S = B \\) |
| `\\[ A^T_S = B \\]` | \\[ A^T_S = B \\] |
| `\\( \sqrt{ab} \\)` | \\( \sqrt{ab} \\) |
| `\\[ \sqrt{ab} \\]` | \\[ \sqrt{ab} \\] |

_html `<table>`_

<table style="width:100%; font-family: monospace;">
<tr>
  <th>Expression</th>
  <th>Rendering</th>
</tr>
<tr>
  <td>`\\(A^T_S = B\\)`</td>
  <td>\\(A^T_S = B\\)</td>
</tr>
<tr>
  <td>`\\[A^T_S = B\\]`</td>
  <td>\\[A^T_S = B\\]</td>
</tr>
</table>

_`<div>`_

<div>\\(A^T_S = B\\)</div>    
<div>\\[A^T_S = B\\]</div>  

----------

**Expression Syntax: `\(…\), \[…\]`**  

`\(A^T_S = B\)` --> \(A^T_S = B\)  
`\[A^T_S = B\]` --> \[A^T_S = B\]  
`\(\sqrt{ab}\)` --> \(\sqrt{ab}\)  
`\[\sqrt{ab}\]` --> \[\sqrt{ab}\]  

_Pipe Table_

|   Expression    |   Rendering   |
| :-------------: | :-----------: |
| `\(A^T_S = B\)` | \(A^T_S = B\) |
| `\[A^T_S = B\]` | \[A^T_S = B\] |
| `\(\sqrt{ab}\)` | \(\sqrt{ab}\) |
| `\[\sqrt{ab}\]` | \[\sqrt{ab}\] |

_html `<table>`_

<table style="width:100%; font-family: monospace;">
<tr>
  <th>Expression</th>
  <th>Rendering</th>
</tr>
<tr>
  <td>`\(A^T_S = B\)`</td>
  <td>\(A^T_S = B\)</td>
</tr>
<tr>
  <td>`\[A^T_S = B\]`</td>
  <td>\[A^T_S = B\]</td>
</tr>
</table>

_`<div>`_

<div>\(A^T_S = B\)</div>    
<div>\[A^T_S = B\]</div>  

----------
