# 拉普拉斯变换

## Formal definition

$$F(s)=\int_0^\infty f(t)e^{-st}dt$$

where s is a complex frequency domain parameter: ${\displaystyle s=\sigma +i\omega ,}$, with real numbers σ and ω.

An alternate notation for the Laplace transform is $ \mathcal {L}\{f\} $ instead of F.

## 常用拉普拉斯变换

参考自 Control Systems Engineering 7th Ed - Nise. chapter 2

1、 $L[\delta(t)] = 1$

2、 $L[u(t)] = \dfrac{1}{s}$

3、 $L[tu(t)] = \dfrac{1}{s^2}$

4、 $L[t^nu(t)] = \dfrac{n!}{s^{n+1}}$

5、 $L[e^{-at}u(t)] = \dfrac{1}{s+a}$

6、 $L[sin(\omega t)u(t)] = \dfrac{\omega}{s^2 + \omega ^2}$

7、 $L[cos(\omega t)u(t)] = \dfrac{s}{s^2 + \omega ^2}$

补充：

1、 $L[te^{-at}u(t)] = \dfrac{1}{(s+a)^2}$

证明1、

方法1：证明之前必须要了解冲激函数的定义和性质，这里先看冲击函数的定义和采样性质。定义：

$$\begin{aligned}\delta(t)=\left\{\begin{array}{cc}+\infty&t=0\\0&t\neq0\end{array}\right.\end{aligned}$$

$$\begin{aligned}\int_{-\infty}^{+\infty}\delta(t)\mathrm{d}t=1\end{aligned}$$

采样性质：根据$\delta$函数的定义，如果他与任意函数相乘，那么相乘的结果只有在脉冲处有值，其他地方的值为0。相乘积分后有这样的结论： $\int_{-\infty}^{+\infty}\delta(t)x(t)\mathrm{d}t=x(0)$, 如果将δ函数平移到$t_0$处，那么对应的，$x(t)$也是在$t_0$时刻的瞬时值会被取出：$\int_{-\infty}^{+\infty}\delta(t-t_0)x(t)\mathrm{d}t=x(t_0)$

那么根据
$$
\begin{aligned}
L[\delta(t)] &= \int_{0-}^{\infty}\delta(t)e^{-st}dt\\
&= \int_{-\infty}^{\infty}\delta(t)e^{-st}dt\\
&= e^{-st}|_{t=t_0=0}\\
&= 1
\end{aligned}
$$

*方法2、方法3是 Gemini-Pro 人工智能给的证明。*

方法2：或从$\delta(t)$的定义来证明，由于 $\delta(t)$ 在 $t=0$ 以外处处为零，因此积分中只有 $t=0$ 处的贡献。将 $\delta(t)$ 的定义代入积分，得到：

$$
\begin{aligned}
L[\delta(t)] &= \int_{0^-}^{\infty}e^{-st}\delta(t)dt\\
&= \lim_{\epsilon \rightarrow 0} \int_{-\epsilon}^\epsilon e^{-st} \delta(t)dt\\
&=e^{-s \cdot 0}\lim_{\epsilon \rightarrow 0} \int_{-\epsilon}^\epsilon \delta(t)dt\\
&=1
\end{aligned}
$$

方法3：冲击函数可以看作是单位阶跃函数的导数，即：

$$\delta(t)= \dfrac{d}{dt}u(t)$$

其中：$u(t)$ 是单位阶跃函数，定义为：

$$
\begin{aligned}
u(t)=\left\{
\begin{array}{cc}
1&t≥0\\
0&t<0
\end{array}\right.
\end{aligned}
$$

由于拉普拉斯变换具有线性性质，因此:

$$
\begin{aligned}
L[\delta(t)] & = L[\dfrac{d}{dt}u(t)]\\
&= sL[u(t)]-u(0)\\
&= s\dfrac{1}{s} - 0
&= 1
\end{aligned}
$$

看起来很奇怪，为什么冲击函数可以看作是单位阶跃函数的导数，为什么$u(0) = 0 $，而不是$u(0) = 1 $

证明2、

$$
\begin{aligned}
L[u(t)] &= \int_{0-}^{\infty}u(t)e^{-st}dt\\
&= \int_{0-}^{\infty}e^{-st}dt\\
&= -\frac{1}{s}e^{-st}|_{0-}^{\infty}\\
&= 0-(-\frac{1}{s})\\
&= \dfrac{1}{s}
\end{aligned}
$$

证明3、

$$
\begin{aligned}
L[tu(t)] &= \int_{0-}^{\infty}tu(t)e^{-st}dt\\
&= -\frac{1}{s}te^{-st}|_{0-}^{\infty} - \int_{0-}^{\infty}(-\frac{1}{s}e^{-st})dt\\
&= \int_{0-}^{\infty}(\frac{1}{s}e^{-st})dt\\
&= \frac{1}{s^2}e^{-st}|_{0-}^{\infty}\\
&= \dfrac{1}{s^2}
\end{aligned}
$$

证明中用到的推导有：$(-\dfrac{1}{s}te^{-st})'=te^{-st} - -\dfrac{1}{s}e^{-st}$

证明4、$L[t^nu(t)] = \dfrac{n!}{s^{n+1}}$

TODO

证明5、$L[e^{-at}u(t)] = \dfrac{1}{s+a}$

$$
\begin{aligned}
L[e^{-at}u(t)] &= \int_{0-}^{\infty}e^{-at}e^{-st}dt\\
&= \int_{0-}^{\infty}e^{-(a+s)t}dt\\
&= -\dfrac{1}{a+s}e^{-(a+s)t}|_{0-}^{\infty}\\
&= \dfrac{1}{s+a}
\end{aligned}
$$

证明6、（提示，用欧拉公式）$L[sin(\omega t)u(t)] = \dfrac{\omega}{s^2 + \omega ^2}$

根据欧拉公式：$e^{ix} = \cos x + i\sin x$, 得到$e^{-ix} = \cos x - i\sin x$, 进而得到: $\sin x = \dfrac{e^{ix} - e^{-ix}}{2i}$ 以及 $\cos x = \dfrac{e^{ix}+ e^{-ix}}{2}$

因此：

$$
\begin{aligned}
L[sin(\omega t)u(t)] &= \int_{0-}^{\infty}sin(\omega t)u(t)e^{-st}dt\\
&= \int_{0-}^{\infty}\dfrac{e^{i\omega t} - e^{-i\omega t}}{2i}u(t)e^{-st}dt\\
&= \dfrac{1}{2i}[\int_{0-}^{\infty}(e^{i\omega t} - e^{-i\omega t})u(t)e^{-st}dt]\\
&= \dfrac{1}{2i}[\dfrac{1}{-i\omega +s} -\dfrac{1}{i\omega+s}]\\
&= \dfrac{1}{2i}[\dfrac{(i\omega+s) - (-i\omega +s)}{s^2+\omega^2}]\\
&= \dfrac{i\omega}{s^2+\omega^2}
\end{aligned}
$$

证明7、略！

## 拉普拉斯变换性质<sup>[1]</sup>

参考自[Laplace transform. Wikipedia.](https://en.wikipedia.org/wiki/Laplace_transform)

$$
\begin{array}
{|c|c|c|c|c|c|c|c|c|}
\hline \text{} &\text{Property}&\text{Time domain}&\text{s domain}&\text{Comment}\\
\hdashline \text{1} &\text{Linearity}&af(t)+bg(t)&aF(s)+bG(s)&\text{Can be proved using basic rules of integration.}\\
\hdashline \text{2} & \text{Frequency-domain derivative}&tf(t) & -F'(s) &\text {F' is the first derivat of F with respect to s}\\
\hdashline \text{3} & \text{Frequency-domain general derivative}& t^{n}f(t) & (-1)^{n}F^{(n)}(s) &\text{More general form, nth derivative of F(s).}\\
\hdashline \text{4} & \text{Derivative}& f'(t) & sF(s)-f(0^-) &\text{}\\
\hdashline \text{5} & \text{Second derivative}& f''(t) & s^2F(s)- sf(0^-)-f'(0^-) &\text{}\\
\hdashline \text{6} & \text{General derivative}& f^{(n)}(t) & s^nF(s)-\sum_{k=1}^ns^{n-k}f^{(k-1)}(0^-) &\text{}\\
\hdashline \text{7} & \text{Frequency-domain integration}& \frac{1}{t}f(t) & \int_s^\infty F(\sigma)d\sigma  &\text{}\\
\hdashline \text{8} & \text{Time-domain integration}& \int_0^tf(\tau)d\tau=(u*f)(t) &\dfrac{1}{s}F(s) &\text{}\\
\hdashline \text{9} & \text{Frequency shifting}& e^{at}f(t) & F(s-a) &\text{}\\
\hdashline \text{10} & \text{Time shifting}& f(t-a)u(t-a) & e^{-as}F(s) &\text{}\\
\text{} &\text{} &f(t)u(t-a) & e^{-as}\mathcal{L}\{f(t+a)\} \\
\hdashline \text{11} & \text{Time scaling}& f(at) & \dfrac{1}{a}F\left(\dfrac{s}{a}\right) &\text{}\\
\hdashline \text{12} & \text{Multiplication}& f(t)g(t) & \dfrac1{2\pi i}\lim_{T\to\infty}\int_{c-iT}^{c+iT}F(\sigma)G(s-\sigma)d\sigma &\text{}\\
\hdashline \text{13} & \text{Convolution}& (f*g)(t)=\int_0^tf(\tau)g(t-\tau)d\tau & F(s)\cdot G(s) &\text{}\\
\hdashline \text{14} & \text{Circular convolution}& (f*g)(t)=\int_0^Tf(\tau)g(t-\tau)d\tau & F(s)\cdot G(s) &\text{}\\
\hdashline \text{15} & \text{Complex conjugation}& f^*(t) & F^*(s^*) &\text{}\\
\hdashline \text{16} & \text{Cross-correlation}& (f\star g)(t)=\int_0^\infty f(\tau)^*\left.g(t+\tau)\right.d\tau & F^*(-s^*)\cdot G(s) &\text{}\\
\hdashline \text{17} & \text{Periodic function}& f(t) & \dfrac1{1-e^{-Ts}}\int_0^Te^{-st}f(t)dt &\text{}\\
\hdashline \text{18} & \text{Periodic summation}& f_P(t)=\sum_{n=0}^\infty f(t-Tn) & F_P(s)=\dfrac1{1-e^{-Ts}}F(s) &\text{}\\
\text{} & \text{} & f_P(t)=\sum_{n=0}^\infty(-1)^nf(t-Tn) & F_P(s)=\dfrac1{1+e^{-Ts}}F(s)\\
\hline
\end{array}
$$

### 证明

#### 1、Linearity 线性(证明略！)

Can be proved using basic rules of integration.

#### 2、Frequency-domain derivative.

$F'$ is the first derivative of F with respect to s.

因为

$$ F(s) = \int_{0-}^{\infty}f(t)e^{-st}dt$$

那么

$$
\begin{aligned}
F'(s)&=\int_{0-}^{\infty}[-tf(t)e^{-st}]dt\\
&= \mathcal {L}[-tf(t)]
\end{aligned}
$$

有：$-tf(t)$的拉普拉斯变换为$F'(s)$. 也就是 $ tf(t) \rightarrow -F'(s)$.

#### 3、Frequency-domain general derivative (证明略)

More general form, nth derivative of F(s).

#### 4、Derivative

f is assumed to be a differentiable function, and its derivative is assumed to be of exponential type. This can then be obtained by integration by parts

$$
\begin{aligned}
sF(s) &= s\int_{0^-}^{\infty}f(t)e^{-st}dt\\
&= \int_{0^-}^{\infty}sf(t)e^{-st}dt\\
&= \int_{0^-}^{\infty}\{[-f(t)e^{-st}]' - [-f'(t)e^{-st}]\}dt\\
&= -f(t)e^{-st}|_{0^-}^{\infty} - \int_{0^-}^{\infty}-f'(t)e^{-st}dt\\
&= \int_{0^-}^{\infty}f'(t)e^{-st}dt + f(0^-)\\
&= \mathcal {L}[f'(t)] + f(0^-)
\end{aligned}
$$

可以看出$\mathcal {L}[f'(t)] = sF(s)-f(0^-)$

#### 5、Second derivative

$$
\begin{aligned}
s^2 F(s) &= \int_{0^-}^{\infty}s^2 f(t)e^{-st}dt\\
&= \int_{0^-}^{\infty}\{[-sf(t)e^{-st}]' - [-sf'(t)e^{-st}]\}dt\\
&= - sf(t)e^{-st}|_{0^-}^{\infty} + \int_{0^-}^{\infty}sf'(t)e^{-st}dt \\
&= sf(0^-)
\end{aligned}
$$

上面的证明方法有点不方便。

$$
\begin{aligned}
\mathcal {L}[f''(t)] &= \int_{0^-}^{\infty}f''(t)e^{-st}dt \\
&= \int_{0^-}^{\infty}\{[f'(t)e^{-st}] - [-sf'(t)e^{-st}]\}dt\\
&= -f'(0^-) + \int_{0^-}^{\infty}sf'(t)e^{-st}dt\\
&= -f'(0^-) + \int_{0^-}^{\infty} \{[sf(t)e^{-st}]-[-s^2f(t)e^{-st}]\}dt\\
&= -f'(0^-) -sf(0^-) + s^2\mathcal L[f(t)]\\
&= s^2F(s) -sf(0^-) - f'(0^-)
\end{aligned}
$$

f is assumed twice differentiable and the second derivative to be of exponential type. Follows by applying the Differentiation property to f′(t).

可是，这个性质，这个公式，有什么用？

#### 6、General derivative (证明略)

f is assumed to be n-times differentiable, with nth derivative of exponential type. Follows by [mathematical induction](https://en.wikipedia.org/wiki/Mathematical_induction).

$$\mathcal L[f^{(n)}(t)] = s^nF(s)-\sum_{k=1}^ns^{n-k}f^{(k-1)}(0^-)$$

#### 7、Frequency-domain integration

This is deduced using the nature of frequency differentiation and conditional convergence.

$$\mathcal L[\frac{1}{t}f(t)] = \int_s^\infty F(\sigma)d\sigma $$

证明：

$$
\begin{aligned}
\mathcal{L}[\frac{1}{t}f(t)] = \int_0^\infty \frac{1}{t} f(t) e^{-st} dt
\end{aligned}
$$

令：$u=\dfrac{1}{t}$, $v' = f(t)e^{-st}$, 那么 $u' = -\dfrac{1}{t^2}$, $v = \int_{0^-}^{t}f(t)e^{-st}dt$

那么：

$$
\begin{aligned}
\int_0^\infty \frac{1}{t} f(t) e^{-st} dt &= \int_0^\infty uv' dt \\
&= uv|_{0^-}^{\infty} - \int_0^\infty u'v dt\\
&= .......
\end{aligned}
$$

<font fa.ce="黑体" color=red >尚待证明</font>

$$\lim_{t \to \infty} \frac{1}{t} \left[ -F(s) / s \right] = 0$$

#### 8、Time-domain integration

$u(t)$ is the Heaviside step function and $(u ∗ f)(t)$ is the convolution of $u(t)$ and $f(t)$.

证明：$\mathcal L[\frac{1}{t}f(t)] = \frac{1}{s}F(s)$

#### 9、Frequency shifting

#### 10、Time shifting

$a > 0$, $u(t)$ is the Heaviside step function

$e^{-as}\mathcal{L}\{f(t+a)\}是否等于 $e^{-as}F(s+a)$？为什么？

#### 11、Time scaling

$a > 0$

#### 12、Multiplication

The integration is done along the vertical line $Re(\sigma) = c$ that lies entirely within the region of convergence of F.

#### 13、Convolution

**写传递函数的时候一直使用该性质**。

证明：$\mathcal L[f(t)*g(t)] = F(s) \cdot G(s)$

$$
\begin{aligned}
\mathcal{L}[(f * g)(t)] &= \int_0^\infty e^{-st}\left(\int_0^t f(\tau)g(t-\tau)d\tau\right)dt\\
&= \int_0^\infty \left(\int_\tau^\infty e^{-st}g(t-\tau)dt\right)f(\tau)d\tau\\
&= \int_0^\infty e^{-s\tau}\left(\int_0^\infty e^{-s(t-\tau)}g(t-\tau)dt\right)f(\tau)d\tau\\
&= \int_0^\infty e^{-s\tau}f(\tau)\left(\int_0^\infty e^{-st}g(t)dt\right)d\tau\\
&= \int_0^\infty e^{-s\tau}f(\tau)d\tau \cdot \int_0^\infty e^{-st}g(t)dt\\
&= F(s)G(s)
\end{aligned}
$$

在上述推导中，我们首先交换了积分顺序，然后对内层积分做变量替换 $t=t-\tau+\tau$。接着我们利用了拉普拉斯变换的线性性质，将两个积分分开。最后根据拉普拉斯变换的定义，我们得到了结果 $\mathcal{L}[(f * g)(t)] = F(s)G(s)$。

因此，我们证明了卷积的拉普拉斯变换等于两个函数拉普拉斯变换的乘积。这个重要的性质在求解线性常微分方程和信号处理等领域有广泛应用。

#### 14、Circular convolution

For periodic functions with period T.

#### 15、Complex conjugation 共轭复数

#### 16、Cross-correlation

what is the mean of star operator? 公式中的五角星是什么运算符，五角星号和\*是怎样区分的，英文中又如何分别描述？

#### 17、Periodic function

$f(t)$ is a periodic function of period T so that $f(t) = f(t + T)$, for all $t ≥ 0$. This is the result of the time shifting property and the [geometric series](https://en.wikipedia.org/wiki/Geometric_series).

#### 18、Periodic summation

## 参考及引用

[1] Laplace transform. Wikipedia. <https://en.wikipedia.org/wiki/Laplace_transform>
[2] <https://sciencedirect.com/topics/mathematics/laplace-transform>
